Complete taifol proof

raft/proof/TermsAndIndicesFromOneLogProof.v
@@ -6,8 +6,8 @@ Require Import Util.
 Require Import Net.
 
 Require Import Raft.
-Require Import RaftRefinementInterface.
 Require Import CommonDefinitions.
+Require Import CommonTheorems.
 Require Import SpecLemmas.
 
 Require Import UpdateLemmas.
@@ -22,11 +22,21 @@ Section TermsAndIndicesFromOneLog.
   Context {raft_params : RaftParams orig_base_params}.
   Context {ctgzi : current_term_gt_zero_interface}.
 
-  Lemma terms_and_indices_from_one_log_init :
-    raft_net_invariant_init terms_and_indices_from_one_log.
+  Definition terms_and_indices_from_one_log_nw (net : network) : Prop :=
+    forall p t leaderId prevLogIndex prevLogTerm entries leaderCommit,
+      In p (nwPackets net) ->
+      pBody p = AppendEntries t leaderId prevLogIndex prevLogTerm entries leaderCommit ->
+      terms_and_indices_from_one entries.
+
+  Definition terms_and_indices_from_one_log_ind (net : network) : Prop :=
+    terms_and_indices_from_one_log net /\ terms_and_indices_from_one_log_nw net.
+
+  Lemma terms_and_indices_from_one_log_ind_init :
+    raft_net_invariant_init terms_and_indices_from_one_log_ind.
   Proof.
-    unfold raft_net_invariant_init, terms_and_indices_from_one_log.
-    unfold terms_and_indices_from_one. simpl. contradiction.
+    split.
+    - unfold terms_and_indices_from_one_log, terms_and_indices_from_one. simpl. contradiction.
+    - unfold terms_and_indices_from_one_log_nw, terms_and_indices_from_one. simpl. contradiction.
   Qed.
 
   Ltac update_destruct :=
@@ -35,118 +45,171 @@ Section TermsAndIndicesFromOneLog.
       | [ H : context [ update _ ?y _ ?x ] |- _ ] => destruct (name_eq_dec y x)
     end.
 
-  Lemma terms_and_indices_from_one_log_client_request :
-    raft_net_invariant_client_request terms_and_indices_from_one_log.
+  Lemma taifol_no_append_entries :
+    forall ps' net ms p t leaderId prevLogIndex prevLogTerm entries leaderCommit h,
+      (forall (p : packet), In p ps' -> In p (nwPackets net) \/ In p (send_packets h ms)) ->
+      (forall m, In m ms -> ~ is_append_entries (snd m)) ->
+      In p ps' ->
+      pBody p = AppendEntries t leaderId prevLogIndex prevLogTerm entries leaderCommit ->
+      terms_and_indices_from_one_log_nw net ->
+      terms_and_indices_from_one entries.
   Proof.
-    unfold raft_net_invariant_client_request, terms_and_indices_from_one_log.
-    simpl. intuition. find_higher_order_rewrite. update_destruct; subst; rewrite_update.
-    - find_apply_lem_hyp handleClientRequest_log. intuition.
+    intros. find_apply_hyp_hyp. break_or_hyp; eauto. unfold send_packets in *. do_in_map.
+    find_apply_hyp_hyp. unfold not in *. find_false.
+    subst. simpl in *. repeat find_rewrite. eauto 10.
+  Qed.
+
+  Lemma terms_and_indices_from_one_log_ind_client_request :
+    raft_net_invariant_client_request terms_and_indices_from_one_log_ind.
+  Proof.
+    red. unfold terms_and_indices_from_one_log_ind. split; red; simpl in *; intuition.
+    - find_higher_order_rewrite. update_destruct; subst; rewrite_update; auto.
+      find_apply_lem_hyp handleClientRequest_log. intuition.
       + repeat find_rewrite. auto.
-      + break_exists. intuition. unfold terms_and_indices_from_one in *.
+      + break_exists. intuition.
+        unfold terms_and_indices_from_one_log, terms_and_indices_from_one in *.
         intros. repeat find_rewrite. simpl in *. break_or_hyp.
-        * intuition. find_apply_lem_hyp current_term_gt_zero_invariant.
-          find_rewrite. eapply_prop current_term_gt_zero. congruence.
+        * intuition. find_apply_lem_hyp current_term_gt_zero_invariant. find_rewrite.
+          eapply_prop current_term_gt_zero. congruence.
         * eauto.
+    - eapply taifol_no_append_entries; eauto using handleClientRequest_no_append_entries.
+  Qed.
+
+  Lemma terms_and_indices_from_one_log_ind_timeout :
+    raft_net_invariant_timeout terms_and_indices_from_one_log_ind.
+  Proof.
+    red. unfold terms_and_indices_from_one_log_ind. split; red; simpl in *; intuition.
+    - find_higher_order_rewrite. update_destruct; subst; rewrite_update; auto.
+      find_apply_lem_hyp handleTimeout_log_same. find_rewrite. auto.
+    - eapply taifol_no_append_entries; eauto using handleTimeout_packets.
+  Qed.
+
+  Lemma terms_and_indices_from_one_app :
+    forall xs ys,
+      terms_and_indices_from_one xs ->
+      terms_and_indices_from_one ys ->
+      terms_and_indices_from_one (xs ++ ys).
+  Proof.
+    induction xs.
     - auto.
+    - unfold terms_and_indices_from_one in *. simpl. intros. break_or_hyp; eauto.
   Qed.
 
-  Lemma terms_and_indices_from_one_log_timeout :
-    raft_net_invariant_timeout terms_and_indices_from_one_log.
+  Lemma terms_and_indices_from_one_In :
+    forall (xs ys : list entry),
+      (forall x, In x xs -> In x ys) ->
+      terms_and_indices_from_one ys ->
+      terms_and_indices_from_one xs.
   Proof.
-    unfold raft_net_invariant_timeout, terms_and_indices_from_one_log.
-    simpl. intuition. find_higher_order_rewrite. update_destruct; subst; rewrite_update; auto.
-    find_apply_lem_hyp handleTimeout_log_same. find_rewrite. auto.
+    unfold terms_and_indices_from_one. eauto.
   Qed.
 
-  Lemma terms_and_indices_from_one_log_append_entries :
-    raft_net_invariant_append_entries terms_and_indices_from_one_log.
+  Lemma terms_and_indices_from_one_log_ind_append_entries :
+    raft_net_invariant_append_entries terms_and_indices_from_one_log_ind.
   Proof.
-    unfold raft_net_invariant_append_entries, terms_and_indices_from_one_log.
-    simpl. intuition. find_higher_order_rewrite. update_destruct; subst; rewrite_update; auto.
-    find_apply_lem_hyp handleAppendEntries_log. intuition.
-    - find_rewrite. auto.
-    - subst. unfold terms_and_indices_from_one. admit.
-    - break_exists. intuition. subst. unfold terms_and_indices_from_one in *.
-      intros. find_rewrite. admit.
+    red. unfold terms_and_indices_from_one_log_ind. split; red; simpl in *; intuition.
+    - find_higher_order_rewrite. update_destruct; subst; rewrite_update; auto.
+      find_apply_lem_hyp handleAppendEntries_log. intuition.
+      + find_rewrite. auto.
+      + subst. unfold terms_and_indices_from_one_log_nw in *. eauto.
+      + break_exists. intuition. subst. find_rewrite. apply terms_and_indices_from_one_app.
+        * eauto.
+        * eapply terms_and_indices_from_one_In; [eapply removeAfterIndex_in | eauto].
+    - unfold terms_and_indices_from_one_log_nw in *. find_apply_hyp_hyp. intuition; eauto.
+      find_apply_lem_hyp handleAppendEntries_not_append_entries.
+      exfalso. apply H. repeat eexists. subst. eauto.
   Qed.
 
-  Lemma terms_and_indices_from_one_log_append_entries_reply :
-    raft_net_invariant_append_entries_reply terms_and_indices_from_one_log.
+  Lemma terms_and_indices_from_one_log_ind_append_entries_reply :
+    raft_net_invariant_append_entries_reply terms_and_indices_from_one_log_ind.
   Proof.
-    unfold raft_net_invariant_append_entries_reply, terms_and_indices_from_one_log.
-    simpl. intuition. find_higher_order_rewrite. update_destruct; subst; rewrite_update; auto.
-    find_apply_lem_hyp handleAppendEntriesReply_log. find_rewrite. auto.
+    red. unfold terms_and_indices_from_one_log_ind. split; red; simpl in *; intuition.
+    - find_higher_order_rewrite. update_destruct; subst; rewrite_update; auto.
+      find_apply_lem_hyp handleAppendEntriesReply_log. find_rewrite. auto.
+    - find_apply_hyp_hyp. intuition; eauto. do_in_map.
+      find_apply_lem_hyp handleAppendEntriesReply_packets; eauto. subst. contradiction.
   Qed.
 
-  Lemma terms_and_indices_from_one_log_request_vote :
-    raft_net_invariant_request_vote terms_and_indices_from_one_log.
+  Lemma terms_and_indices_from_one_log_ind_request_vote :
+    raft_net_invariant_request_vote terms_and_indices_from_one_log_ind.
   Proof.
-    unfold raft_net_invariant_request_vote, terms_and_indices_from_one_log.
-    simpl. intuition. find_higher_order_rewrite. update_destruct; subst; rewrite_update; auto.
-    find_apply_lem_hyp handleRequestVote_log. find_rewrite. auto.
+    red. unfold terms_and_indices_from_one_log_ind. split; red; simpl in *; intuition.
+    - find_higher_order_rewrite. update_destruct; subst; rewrite_update; auto.
+      find_apply_lem_hyp handleRequestVote_log. find_rewrite. auto.
+    - find_apply_hyp_hyp. intuition; eauto. find_apply_lem_hyp handleRequestVote_no_append_entries.
+      unfold not in *. find_false. repeat eexists. subst. eauto.
   Qed.
 
-  Lemma terms_and_indices_from_one_log_request_vote_reply :
-    raft_net_invariant_request_vote_reply terms_and_indices_from_one_log.
+  Lemma terms_and_indices_from_one_log_ind_request_vote_reply :
+    raft_net_invariant_request_vote_reply terms_and_indices_from_one_log_ind.
   Proof.
-    unfold raft_net_invariant_request_vote_reply, terms_and_indices_from_one_log.
-    simpl. intuition. find_higher_order_rewrite. update_destruct; rewrite_update; auto.
-    symmetry in H. find_apply_lem_hyp handleRequestVoteReply_log. subst. find_rewrite. auto.
+    red. unfold terms_and_indices_from_one_log_ind. split; red; simpl in *; intuition.
+    - find_higher_order_rewrite. update_destruct; rewrite_update; auto.
+      symmetry in H. find_apply_lem_hyp handleRequestVoteReply_log. subst. find_rewrite. auto.
+    - eauto.
   Qed.
 
-  Lemma terms_and_indices_from_one_log_do_leader :
-    raft_net_invariant_do_leader terms_and_indices_from_one_log.
+  Lemma terms_and_indices_from_one_log_ind_do_leader :
+    raft_net_invariant_do_leader terms_and_indices_from_one_log_ind.
   Proof.
-    unfold raft_net_invariant_do_leader, terms_and_indices_from_one_log.
-    simpl. intuition. find_higher_order_rewrite. update_destruct; subst; rewrite_update; auto.
-    find_apply_lem_hyp doLeader_log. find_rewrite. auto.
+    red. unfold terms_and_indices_from_one_log_ind. split; red; simpl in *; intuition.
+    - find_higher_order_rewrite. update_destruct; subst; rewrite_update; auto.
+      find_apply_lem_hyp doLeader_log. find_rewrite. auto.
+    - find_apply_hyp_hyp. intuition; eauto.
+      unfold doLeader in *. repeat break_match; tuple_inversion; subst; try contradiction.
+      repeat do_in_map. unfold replicaMessage in *. subst. simpl in *. find_inversion.
+      eapply terms_and_indices_from_one_In. apply findGtIndex_in. auto.
   Qed.
 
-  Lemma terms_and_indices_from_one_log_do_generic_server :
-    raft_net_invariant_do_generic_server terms_and_indices_from_one_log.
+  Lemma terms_and_indices_from_one_log_ind_do_generic_server :
+    raft_net_invariant_do_generic_server terms_and_indices_from_one_log_ind.
   Proof.
-    unfold raft_net_invariant_do_generic_server, terms_and_indices_from_one_log.
-    simpl. intuition. find_higher_order_rewrite. update_destruct; subst; rewrite_update; auto.
-    find_apply_lem_hyp doGenericServer_log. find_rewrite. auto.
+    red. unfold terms_and_indices_from_one_log_ind. split; red; simpl in *; intuition.
+    - find_higher_order_rewrite. update_destruct; subst; rewrite_update; auto.
+      find_apply_lem_hyp doGenericServer_log. find_rewrite. auto.
+    - find_apply_lem_hyp doGenericServer_packets. find_apply_hyp_hyp. subst. intuition; eauto.
+      do_in_map. contradiction.
   Qed.
 
-  Lemma terms_and_indices_from_one_log_state_same_packet_subset :
-    raft_net_invariant_state_same_packet_subset terms_and_indices_from_one_log.
+  Lemma terms_and_indices_from_one_log_ind_state_same_packet_subset :
+    raft_net_invariant_state_same_packet_subset terms_and_indices_from_one_log_ind.
   Proof.
-    unfold raft_net_invariant_state_same_packet_subset, terms_and_indices_from_one_log.
-    simpl. intuition. find_reverse_higher_order_rewrite. auto.
+    red. unfold terms_and_indices_from_one_log_ind. split; red; simpl in *; intuition.
+    - find_reverse_higher_order_rewrite. auto.
+    - eauto.
   Qed.
 
-  Lemma terms_and_indices_from_one_log_reboot :
-    raft_net_invariant_reboot terms_and_indices_from_one_log.
+  Lemma terms_and_indices_from_one_log_ind_reboot :
+    raft_net_invariant_reboot terms_and_indices_from_one_log_ind.
   Proof.
-    unfold raft_net_invariant_reboot, terms_and_indices_from_one_log.
-    simpl. intuition. find_higher_order_rewrite. update_destruct; subst; rewrite_update; auto.
-    unfold reboot. simpl. auto.
+    red. unfold terms_and_indices_from_one_log_ind. split; red; simpl in *; intuition.
+    - find_higher_order_rewrite. update_destruct; subst; rewrite_update; auto.
+      unfold reboot. eauto.
+    - find_reverse_rewrite. eauto.
   Qed.
 
-  Lemma terms_and_indices_from_one_log_invariant :
+  Lemma terms_and_indices_from_one_log_ind_invariant :
     forall net,
       raft_intermediate_reachable net ->
-      terms_and_indices_from_one_log net.
+      terms_and_indices_from_one_log_ind net.
   Proof.
     intros.
     apply raft_net_invariant; auto.
-    - apply terms_and_indices_from_one_log_init.
-    - apply terms_and_indices_from_one_log_client_request.
-    - apply terms_and_indices_from_one_log_timeout.
-    - apply terms_and_indices_from_one_log_append_entries.
-    - apply terms_and_indices_from_one_log_append_entries_reply.
-    - apply terms_and_indices_from_one_log_request_vote.
-    - apply terms_and_indices_from_one_log_request_vote_reply.
-    - apply terms_and_indices_from_one_log_do_leader.
-    - apply terms_and_indices_from_one_log_do_generic_server.
-    - apply terms_and_indices_from_one_log_state_same_packet_subset.
-    - apply terms_and_indices_from_one_log_reboot.
+    - apply terms_and_indices_from_one_log_ind_init.
+    - apply terms_and_indices_from_one_log_ind_client_request.
+    - apply terms_and_indices_from_one_log_ind_timeout.
+    - apply terms_and_indices_from_one_log_ind_append_entries.
+    - apply terms_and_indices_from_one_log_ind_append_entries_reply.
+    - apply terms_and_indices_from_one_log_ind_request_vote.
+    - apply terms_and_indices_from_one_log_ind_request_vote_reply.
+    - apply terms_and_indices_from_one_log_ind_do_leader.
+    - apply terms_and_indices_from_one_log_ind_do_generic_server.
+    - apply terms_and_indices_from_one_log_ind_state_same_packet_subset.
+    - apply terms_and_indices_from_one_log_ind_reboot.
   Qed.
 
   Instance taifoli : terms_and_indices_from_one_log_interface.
   Proof.
-    split. apply terms_and_indices_from_one_log_invariant.
+    split. apply terms_and_indices_from_one_log_ind_invariant.
   Qed.
 End TermsAndIndicesFromOneLog.
