raft/SpecLemmas.v
@@ -381,6 +381,16 @@ Section SpecLemmas.
     subst; auto.
   Qed.
 
+  Theorem handleAppendEntries_not_append_entries :
+    forall h st t n pli plt es ci st' m,
+      handleAppendEntries h st t n pli plt es ci = (st', m) ->
+      ~ is_append_entries m.
+  Proof.
+    intros. unfold handleAppendEntries in *.
+    repeat break_match; find_inversion;
+    intuition; break_exists; congruence.
+  Qed.
+
   Lemma handleRequestVote_no_append_entries :
     forall st h h' t lli llt st' m,
       handleRequestVote h st t h' lli llt = (st', m) ->
